Main.lean
@@ -1,0 +1,10 @@
+import RakeSieve
+
+
+def main : IO Unit := do
+  let mut s : PrimeSieve _ := { state := RakeSieve.init }
+  for _ in [0:5] do
+    IO.println <| s.state.p
+    s := s.next
+
+#eval main
